Almost wrote append_left

pulse/examples/steel/Selectors.Tree.fsti
@@ -1,108 +1,10 @@
 module Selectors.Tree
 
+open Selectors.Tree.Core
 open Steel.Memory
 open Steel.SelEffect
 
 module Spec = FStar.Trees
-
-(*** Type declarations *)
-
-(**** Base types *)
-
-(** A node of the tree *)
-val node (a: Type0) : Type
-
-(** A tree is a ref to a node, themselves referencing other nodes *)
-let t (a: Type0) = ref (node a)
-
-(** This type reflects the contents of a tree without the memory layout *)
-type tree (a: Type0) = Spec.tree a
-(**** Slprop and selector *)
-
-(** The separation logic proposition representing the memory layout of the tree *)
-val tree_sl (#a: Type0) (r: t a) : slprop u#1
-
-(** Selector retrieving the contents of a tree in memory *)
-val tree_sel (#a: Type0) (r: t a) : selector (tree a) (tree_sl r)
-
-[@@__steel_reduce__]
-let linked_tree' (#a: Type0) (r: t a) : vprop' = {
-  hp = tree_sl r;
-  t = tree a;
-  sel = tree_sel r
-}
-
-(** The view proposition encapsulating the separation logic proposition and the selector *)
-unfold let linked_tree (#a: Type0) (tr: t a) : vprop = VUnit (linked_tree' tr)
-
-(** This convenience helper retrieves the contents of a tree from an [rmem] *)
-[@@ __steel_reduce__]
-let v_linked_tree
-  (#a:Type0)
-  (#p:vprop)
-  (r:t a)
-  (h:rmem p{
-    FStar.Tactics.with_tactic selector_tactic (can_be_split p (linked_tree r) /\ True)
-  })
-    : GTot (tree a)
-  = h (linked_tree r)
-
-(*** Operations *)
-
-(**** Operations on nodes *)
-
-val get_left (#a: Type0) (n: node a) : t a
-val get_right (#a: Type0) (n: node a) : t a
-val get_data (#a: Type0) (n: node a) : a
-val mk_node (#a: Type0) (left right: t a) (v: a)
-    : Pure (node a)
-      (requires True)
-      (ensures (fun n -> get_left n == left /\ get_right n == right /\ get_data n == v))
-
-(**** Low-level operations on trees *)
-
-val null_t (#a: Type0) : t a
-val is_null_t (#a: Type0) (r: t a) : (b:bool{b <==> r == null_t})
-
-val intro_linked_tree_leaf (#a: Type0)
-    : SteelSel unit
-      vemp (fun _ -> linked_tree (null_t #a))
-      (requires (fun _ -> True))
-      (ensures (fun _ _ h1 -> v_linked_tree #a null_t h1 == Spec.Leaf))
-
-val elim_linked_tree_leaf (#a: Type0) (ptr: t a)
-    : SteelSel unit
-       (linked_tree ptr) (fun _ -> linked_tree ptr)
-       (requires (fun _ -> is_null_t ptr))
-       (ensures (fun h0 _ h1 ->
-         v_linked_tree ptr h0 == v_linked_tree ptr h1 /\
-         v_linked_tree ptr h1 == Spec.Leaf))
-
-val pack_tree (#a: Type0) (ptr: t a) (left: t a) (right: t a)
-    : SteelSel unit
-      (vptr ptr `star` linked_tree left `star` linked_tree right)
-      (fun _ -> linked_tree ptr)
-      (requires (fun h0 ->
-        not (is_null_t ptr) /\
-        get_left (sel ptr h0) == left /\
-        get_right (sel ptr h0) == right))
-      (ensures (fun h0 _ h1 ->
-        v_linked_tree ptr h1 ==
-          Spec.Node (get_data (sel ptr h0)) (v_linked_tree left h0) (v_linked_tree right h0)
-      ))
-
-val unpack_tree (#a: Type0) (ptr: t a)
-    : SteelSel (node a)
-      (linked_tree ptr)
-      (fun node ->
-        linked_tree (get_left node) `star` linked_tree (get_right node) `star` vptr ptr)
-      (requires (fun h0 -> not (is_null_t ptr)))
-      (ensures (fun h0 node h1 ->
-        v_linked_tree ptr h0 == Spec.Node
-          (get_data (sel ptr h1))
-          (v_linked_tree (get_left node) h1)
-          (v_linked_tree (get_right node) h1)
-      ))
 
 (**** High-level operations on trees *)
 
