pulse/examples/steel/Selectors.Tree.Core.fst
@@ -1,0 +1,79 @@
+module Selectors.Tree.Core
+
+open Steel.SelEffect
+open Steel.FractionalPermission
+
+module Mem = Steel.Memory
+module R = Steel.Reference
+module Spec = FStar.Trees
+
+#set-options "--fuel 0 --ifuel 1 --z3rlimit 15"
+
+#push-options "--__no_positivity"
+noeq type node (a: Type0) = {
+  data: a;
+  left: ref (node a);
+  right: ref (node a);
+}
+#pop-options
+
+let get_left #a n = n.left
+let get_right #a n = n.right
+let get_data #a n = n.data
+
+let mk_node #a data left right = {
+  data;
+  left;
+  right
+}
+
+let null_t #a = R.null
+let is_null_t #a ptr = R.is_null ptr
+
+let rec tree_sl' (#a: Type0) (ptr: t a) (tree: Spec.tree (node a)) : Tot slprop (decreases tree) =
+  match tree with
+  | Spec.Leaf -> pure (ptr == null_t)
+  | Spec.Node data left right ->
+    R.pts_to ptr full_perm data `Mem.star`
+    tree_sl' data.left left `Mem.star`
+    tree_sl' data.right right `Mem.star`
+    pure (ptr =!= null_t)
+
+let tree_sl #a ptr = Mem.h_exists (tree_sl' ptr)
+
+let rec tree_view (#a: Type0) (tree: Spec.tree (node a)) : Tot (Spec.tree a) (decreases tree) =
+  match tree with
+  | Spec.Leaf -> Spec.Leaf
+  | Spec.Node data left right -> Spec.Node (get_data data) (tree_view left) (tree_view right)
+
+let tree_sel_node' (#a: Type0) (ptr: t a) : selector' (Spec.tree (node a)) (tree_sl ptr) =
+  fun h -> id_elim_exists (tree_sl' ptr) h
+
+let tree_sl'_witinv (#a: Type0) (ptr: t a) : Lemma(is_witness_invariant (tree_sl' ptr))
+  =
+  admit()
+
+let tree_sel_depends_only_on (#a:Type0) (ptr:t a)
+  (m0:Mem.hmem (tree_sl ptr)) (m1:mem{disjoint m0 m1})
+  : Lemma (tree_sel_node' ptr m0 == tree_sel_node' ptr (Mem.join m0 m1))
+  =
+  admit()
+
+let tree_sel_depends_only_on_core (#a:Type0) (ptr:t a)
+  (m0:Mem.hmem (tree_sl ptr))
+  : Lemma (tree_sel_node' ptr m0 == tree_sel_node' ptr (core_mem m0))
+  =
+  admit()
+
+let tree_sel_node (#a: Type0) (ptr: t a) : selector (Spec.tree (node a)) (tree_sl ptr) =
+  Classical.forall_intro_2 (tree_sel_depends_only_on ptr);
+  Classical.forall_intro (tree_sel_depends_only_on_core ptr);
+  tree_sel_node' ptr
+
+let tree_sel #a r = fun h -> tree_view (tree_sel_node r h)
+
+assume val sladmit (#a:Type)
+            (#[@@framing_implicit] p:pre_t)
+            (#[@@framing_implicit] q:post_t a)
+            (_:unit)
+  : SteelSelF a p q (requires fun _ -> True) (ensures fun _ _ _ -> False)
